proofs/transform/eliminate_algebraic_proofs/eliminate_algebraic_semantics.v
@@ -1,0 +1,367 @@
+(*Prove semantics of rewriteT/F*)
+Require Import Task PatternProofs eliminate_algebraic eliminate_algebraic_context eliminate_algebraic_interp 
+  eliminate_algebraic_typing.
+Set Bullet Behavior "Strict Subproofs".
+
+Lemma dom_cast_inj (dom_aux: sort -> Set) {v1 v2 : sort} (H1 H2: v1 = v2) (d1 d2: domain dom_aux v1):
+  dom_cast dom_aux H1 d1 = dom_cast dom_aux H2 d2 ->
+  d1 = d2.
+Proof.
+  subst. assert (H2 = eq_refl) by (apply UIP_dec, sort_eq_dec). subst.
+  unfold dom_cast; simpl. subst; auto.
+Qed.
+
+Lemma scast_inj_uip {S1 S2: Set} (H1 H2: S1 = S2) (x1 x2: S1):
+  scast H1 x1 = scast H2 x2 ->
+  x1 = x2.
+Proof.
+  subst. simpl. intros Hx1; subst.
+  assert (H2 = eq_refl) by (apply UIP).
+  subst; auto.
+Qed.
+
+Lemma semantic_constr_inj_c {g1 g2} (g1_valid: valid_context g1) (g2_valid: valid_context g2) 
+  {m a c1 c2} (m_in1: mut_in_ctx m g1) (m_in2: mut_in_ctx m g2) (a_in: adt_in_mut a m)
+  (c1_in: constr_in_adt c1 a) (c2_in: constr_in_adt c2 a)
+  {args} (args_len: length args = length (m_params m))
+  (pd: pi_dom)
+  (pdf1: pi_dom_full g1 pd) (pdf2: pi_dom_full g2 pd)
+  (vt: typevar -> sort)
+  (d : domain (dom_aux pd) (v_subst vt (vty_cons (adt_name a) args)))
+  (al1: arg_list (domain (dom_aux pd)) (sym_sigma_args c1 (map (v_subst vt) args)))
+  (al2:  arg_list (domain (dom_aux pd)) (sym_sigma_args c2 (map (v_subst vt) args)))
+  (Hsem1: semantic_constr g1_valid pd pdf1 vt m_in1 a_in c1_in args_len d al1)
+  (Hsem2: semantic_constr g2_valid pd pdf2 vt m_in2 a_in c2_in args_len d al2):
+  c1 = c2.
+Proof.
+  unfold semantic_constr in Hsem1, Hsem2.
+  subst.
+  (*Get that constr_reps equal*)
+  apply dom_cast_inj in Hsem2.
+  apply scast_inj_uip in Hsem2.
+  destruct (funsym_eq_dec c1 c2); subst; auto.
+  erewrite constr_rep_change_gamma in Hsem2.
+  apply constr_rep_disjoint in Hsem2; auto. contradiction.
+Qed.
+
+Lemma semantic_constr_inj_al {g1 g2} (g1_valid: valid_context g1) (g2_valid: valid_context g2) 
+  {m a c} (m_in1: mut_in_ctx m g1) (m_in2: mut_in_ctx m g2) (a_in: adt_in_mut a m)
+  (c_in: constr_in_adt c a)
+  {args} (args_len: length args = length (m_params m))
+  (pd: pi_dom)
+  (pdf1: pi_dom_full g1 pd) (pdf2: pi_dom_full g2 pd)
+  (vt: typevar -> sort)
+  (d : domain (dom_aux pd) (v_subst vt (vty_cons (adt_name a) args)))
+  (al1: arg_list (domain (dom_aux pd)) (sym_sigma_args c (map (v_subst vt) args)))
+  (al2:  arg_list (domain (dom_aux pd)) (sym_sigma_args c (map (v_subst vt) args)))
+  (Hsem1: semantic_constr g1_valid pd pdf1 vt m_in1 a_in c_in args_len d al1)
+  (Hsem2: semantic_constr g2_valid pd pdf2 vt m_in2 a_in c_in args_len d al2):
+  al1 = al2.
+Proof.
+  unfold semantic_constr in Hsem1, Hsem2.
+  subst.
+  (*Get that constr_reps equal*)
+  apply dom_cast_inj in Hsem2.
+  apply scast_inj_uip in Hsem2.
+  erewrite constr_rep_change_gamma in Hsem2.
+  apply constr_rep_inj in Hsem2; subst; auto.
+  apply (gamma_all_unif g1_valid _ m_in1).
+Qed.
+
+From Equations Require Import Equations. (*for [simp]*)
+
+Lemma matches_row_vars_eq {g1 g2} (g1_valid: valid_context g1) (g2_valid: valid_context g2) 
+  (pd: pi_dom)
+  (pdf1: pi_dom_full g1 pd) (pdf2: pi_dom_full g2 pd)
+  (vt: val_typevar) (vars: list vsymbol) (tys: list vty)
+  (Hvarsty1 Hvarsty2 : row_typed tys (map Pvar vars))
+  (a : arg_list (domain (dom_aux pd)) (map (v_subst vt) tys)):
+  matches_row g1_valid pd pdf1 vt tys a (map Pvar vars) Hvarsty1 =
+  matches_row g2_valid pd pdf2 vt tys a (map Pvar vars) Hvarsty2.
+Proof.
+  revert Hvarsty1 Hvarsty2. revert vars.
+  induction tys as [| ty1 tys IH]; simpl; intros [| var1 vars] Hty1 Hty2;
+  try solve[inversion Hty1]; [reflexivity|]. simpl.
+  simp matches_row.
+  simpl. erewrite IH. reflexivity.
+Qed.
+
+ 
+(*For a simple pattern, if we match on an element of a type ADT in both contexts, the result is the same*)
+Lemma match_val_single_simple_eq {g1 g2} (g1_valid: valid_context g1) (g2_valid: valid_context g2) 
+  {m a} (m_in1: mut_in_ctx m g1) (m_in2: mut_in_ctx m g2) (a_in: adt_in_mut a m)
+  {args} (args_len: length args = length (m_params m))
+  (pd: pi_dom)
+  (pdf1: pi_dom_full g1 pd) (pdf2: pi_dom_full g2 pd)
+  (vt: typevar -> sort)
+  (ty1: vty) (Htyeq: ty1 = vty_cons (adt_name a) args) (d : domain (dom_aux pd) (v_subst vt ty1)) 
+  (p: pattern) (Hty1: pattern_has_type g1 p ty1) (Hty2: pattern_has_type g2 p ty1)
+  (Hsimp: simple_pat p):
+  match_val_single g1_valid pd pdf1 vt ty1 p Hty1 d =
+  match_val_single g2_valid pd pdf2 vt ty1 p Hty2 d.
+Proof.
+  (*We could prove inductively, but this is painful and we do not. Instead, we use [tm_semantic_constr]
+    and the existing proofs from PatternProofs.v
+    Idea: we have simple_pat, so either a constructor(vars) or wildcard.
+    In second case, both match trivially
+    In first case, we have term of ADT, so get semantic constr c1 and c2 for each.
+    If {c1, c2} match c, then vars match (use [match_val_single_constr_row]). 
+    If either one is not equal, get None by
+    [match_val_single_constr_nomatch]*)
+  destruct p as [| f1 tys1 pats1 | | |]; try discriminate; [|reflexivity].
+  apply simpl_constr_get_vars in Hsimp. destruct Hsimp as [vars Hpats1]; subst pats1.
+  (*Get semantic_constrs*)
+  subst ty1.
+  destruct (find_semantic_constr g1_valid pd pdf1 vt m_in1 a_in args_len d) as [c1 [[c1_in a1] Hsem1]].
+  destruct (find_semantic_constr g2_valid pd pdf2 vt m_in2 a_in args_len d) as [c2 [[c2_in a2] Hsem2]].
+  simpl in Hsem1, Hsem2.
+  (*Need for [match_val_single_constr_row]*)
+  assert (Heq2: sym_sigma_args c2 (map (v_subst vt) args) =
+    map (v_subst vt) (ty_subst_list (s_params c2) args (s_args c2))).
+  {
+    apply sym_sigma_args_map. rewrite (adt_constr_params g2_valid m_in2 a_in c2_in); auto.
+  }
+  assert (Htys: tys1 = args). {
+    eapply constr_pattern_is_constr in Hty1; eauto. destruct_all; auto.
+  }
+  subst tys1.
+  assert (Hvarsty1: @row_typed g1 (ty_subst_list (s_params f1) args (s_args f1)) (map Pvar vars))
+    by (apply constr_typed_row in Hty1; auto).
+  assert (Hvarsty2: @row_typed g2 (ty_subst_list (s_params f1) args (s_args f1)) (map Pvar vars))
+    by (apply constr_typed_row in Hty2; auto).
+  (*Know c1 and c2 are equal*)
+  assert (Hc12: c1 = c2). { eapply (semantic_constr_inj_c g1_valid g2_valid); eauto. }
+  subst c1.
+  destruct (funsym_eq_dec f1 c2); subst.
+  - (*If both equal, then both match all*)
+    rewrite (match_val_single_constr_row g1_valid pd pdf1 vt m_in1 a_in c1_in args_len d a1 Hsem1 _ _ Hty1 Heq2 Hvarsty1).
+    rewrite (match_val_single_constr_row g2_valid pd pdf2 vt m_in2 a_in c2_in args_len d a2 Hsem2 _ _ Hty2 Heq2 Hvarsty2).
+    assert (c1_in = c2_in) by (apply bool_irrelevance); subst.
+    assert (a1 = a2). { eapply (semantic_constr_inj_al g1_valid g2_valid); eauto. }
+    subst a2.
+    apply matches_row_vars_eq.
+  - erewrite !match_val_single_constr_nomatch; eauto.
+Qed.
+
+
+(*For a list of simple patterns, we can change the context assuming the type is in both*)
+Lemma match_rep_simple {g1 g2} (g1_valid: valid_context g1) (g2_valid: valid_context g2) 
+  {m a} (m_in1: mut_in_ctx m g1) (m_in2: mut_in_ctx m g2) (a_in: adt_in_mut a m)
+  {args} (args_len: length args = length (m_params m))
+  (pd: pi_dom)
+  (pdf1: pi_dom_full g1 pd) (pdf2: pi_dom_full g2 pd) (pf1: pi_funpred g1_valid pd pdf1)
+  (pf2: pi_funpred g2_valid pd pdf2) (vt: typevar -> sort) (vv: val_vars pd vt) (b1: bool)
+  (ty: gen_type b1) (ty1: vty) (Hty1: ty1 = vty_cons (adt_name a) args) (d : domain (dom_aux pd) (v_subst vt ty1)) 
+  (pats1: list (pattern * gen_term b1)) (pats2: list (pattern * gen_term b1))
+  (Hpatsfst: map fst pats1 = map fst pats2)
+  (Hpatsnd: Forall2 (fun (t1 t2 : gen_term b1) => forall Hty1 Hty2 vv, 
+    gen_rep g1_valid pd pdf1 pf1 vt vv ty t1 Hty1 =
+    gen_rep g2_valid pd pdf2 pf2 vt vv ty t2 Hty2) (map snd pats1) (map snd pats2))
+  (Hpats1 : Forall (fun x => pattern_has_type g1 (fst x) ty1) pats1)
+  (Hpats2 : Forall (fun x => gen_typed g1 b1 (snd x) ty) pats1)
+  (Hpats3 : Forall (fun x  => pattern_has_type g2 (fst x) ty1) pats2)
+  (Hpats4 : Forall (fun x => gen_typed g2 b1 (snd x) ty) pats2)
+  (Hallsimp: forallb simple_pat (map fst pats1)) (*TODO: do we need simple_exhaust?*):
+  match_rep g1_valid pd pdf1 vt vv (term_rep g1_valid pd pdf1 vt pf1)
+    (formula_rep g1_valid pd pdf1 vt pf1) b1 ty ty1 d pats1 Hpats1 Hpats2 =
+  match_rep g2_valid pd pdf2 vt vv (term_rep g2_valid pd pdf2 vt pf2)
+    (formula_rep g2_valid pd pdf2 vt pf2) b1 ty ty1 d pats2 Hpats3 Hpats4.
+Proof.
+  rewrite !match_rep_equiv. (*use gen_rep now*)
+  generalize dependent pats2. generalize dependent pats1. induction pats1 as [|[p1 t1] ptl1 IH]; simpl;
+  intros Hpats1 Hpats1' Hsimp [| [p2 t2] ptl2]; auto; try discriminate.
+  simpl. intros Hfst Hsnd Hpats2 Hpats2'. simpl.
+  injection Hfst. intros Hfst' Hp12; subst p2. apply andb_true_iff in Hsimp; destruct Hsimp as [Hsimp1 Hsimp2].
+  inversion Hsnd; subst.
+  rewrite (match_val_single_simple_eq g1_valid g2_valid m_in1 m_in2 a_in args_len) with (pdf2:=pdf2)
+    (Hty2:=(Forall_inv Hpats2)); auto; simpl.
+  destruct (match_val_single g2_valid pd pdf2 vt _ p1 (Forall_inv Hpats2) d ) eqn : Hmatch1; auto.
+Qed.
+
+
+Section Proofs.
+
+Variable (keep_muts: mut_adt -> bool) (new_constr_name: funsym -> string)
+  (noind: typesym -> bool) (badvars: list vsymbol).
+
+
+Context {gamma: context} (gamma_valid: valid_context gamma). (*old context*)
+
+(*We already fixed badnames from context*)
+Notation badnames := (idents_of_context gamma).
+
+Local Definition new_gamma := new_ctx new_constr_name keep_muts (idents_of_context gamma) noind gamma.
+Check new_gamma_gen_valid' .
+
+Variable (new_constrs_inj: forall (m1 m2 : mut_adt) (a1 a2 : alg_datatype),
+mut_in_ctx m1 gamma ->
+mut_in_ctx m2 gamma ->
+adt_in_mut a1 m1 ->
+adt_in_mut a2 m2 ->
+forall c1 c2 : funsym,
+constr_in_adt c1 a1 -> constr_in_adt c2 a2 -> new_constr_name c1 = new_constr_name c2 -> c1 = c2).
+
+(*NOTE: for now, just assume new_gamma is valid. We will compose with typing hypotheses later*)
+
+(* Lemma new_gamma_valid: valid_context new_gamma.
+Proof.
+  unfold new_gamma, new_ctx.
+  apply new_gamma_gen_valid'; auto. *)
+
+Variable (new_gamma_valid: valid_context new_gamma).
+Variable (pd: pi_dom) (pdf: pi_dom_full gamma pd) (pf: pi_funpred gamma_valid pd pdf).
+
+(*New pf*)
+Local Definition new_pdf : pi_dom_full new_gamma pd := pd_new_full new_constr_name keep_muts noind pd pdf.
+Local Definition new_pf : pi_funpred new_gamma_valid pd new_pdf :=
+  pf_new new_constr_name keep_muts noind gamma_valid pd pdf pf new_gamma_valid.
+Variable (vt: val_typevar).
+
+Check term_rep.
+Print rewriteT.
+
+(*TODO: why is it impossible to make something opaque*)
+Opaque n_str.
+Opaque under_str.
+
+
+
+Lemma rewrite_rep t f:
+  (forall (ty: vty) (Hty1: term_has_type gamma t ty) 
+    (Hsimp: term_simple_pats t)
+    (Hexh: term_simple_exhaust gamma t)
+    (Hty2: term_has_type new_gamma 
+      (rewriteT keep_muts new_constr_name badnames gamma badvars t) ty) 
+    (vv: val_vars pd vt), 
+    term_rep new_gamma_valid pd new_pdf vt new_pf vv 
+      (rewriteT keep_muts new_constr_name badnames gamma badvars t) ty Hty2 =
+    term_rep gamma_valid pd pdf vt pf vv t ty Hty1) /\
+  (forall (Hty1: formula_typed gamma f)
+    (Hsimp: fmla_simple_pats f)
+    (Hexh: fmla_simple_exhaust gamma f) (av: list vsymbol) (sign: bool) (Hty2: formula_typed new_gamma 
+    (rewriteF keep_muts new_constr_name badnames gamma badvars av sign f)) 
+    (vv: val_vars pd vt), 
+    formula_rep new_gamma_valid pd new_pdf vt new_pf vv 
+      (rewriteF keep_muts new_constr_name badnames gamma badvars av sign f) Hty2 =
+    formula_rep gamma_valid pd pdf vt pf vv f Hty1).
+Proof.
+  (*NOTE: can't use term_formula_ind_typed because dependent, and then we need type info e.g. in functions
+  maybe go back and generalize that, see*)
+  revert t f; apply term_formula_ind.
+  - (*Tconst*) intros. simpl. inversion Hty1; subst; simpl_rep_full; f_equal; apply UIP_dec, vty_eq_dec.
+  - (*Tvar*)  intros. inversion Hty1; subst. simpl_rep_full. f_equal. apply UIP_dec, sort_eq_dec.
+  - (*Tfun*) intros f1 tys tms IH ty Hty1. simpl. unfold is_true; rewrite !forallb_forall.
+    intros Hsimp Hexh Hty2 vv.
+    simpl_rep_full.
+    revert Hty2. simpl. 
+    destruct (f_is_constr f1 && enc_ty keep_muts gamma (f_ret f1)) eqn : Hconstrty; intros Hty2.
+    + (*Case 1: constr*)
+      simpl_rep_full.
+      f_equal; [apply UIP_dec, vty_eq_dec|].
+      apply dom_cast_eq'.
+      (*2 parts: 1. Show that funs equal (bc constr)
+                2. Show that [arg_list] equal (by IH)
+        Do 2nd part first*)
+      assert (Hargs: (fun_arg_list pd vt (new_constr new_constr_name badnames f1) tys
+         (map (rewriteT keep_muts new_constr_name badnames gamma badvars) tms)
+         (term_rep new_gamma_valid pd new_pdf vt new_pf vv) Hty2) = 
+      (fun_arg_list pd vt f1 tys tms (term_rep gamma_valid pd pdf vt pf vv) Hty1)).
+      {
+        apply get_arg_list_ext; [solve_len|].
+        simpl_len. intros i Hi ty1 Hty3 Hty4.
+        revert Hty3.
+        rewrite map_nth_inbound with (d2:=tm_d); auto. intros Hty3.
+        assert (Hin: In (nth i tms tm_d) tms) by (apply nth_In; auto).
+        rewrite Forall_forall in IH. apply IH; auto.
+      }
+      rewrite Hargs; clear Hargs.
+      (*Now prove functions equiv*)
+      destruct (f_is_constr f1) eqn : Hconstr; [|discriminate].
+      apply (is_constr_iff _ gamma_valid) in Hconstr.
+      2: { inversion Hty1; subst; auto. }
+      destruct Hconstr as [m [a [m_in [a_in c_in]]]].
+      (*Now use enc_ty info to show equal*)
+      unfold funs_new_full.
+      rewrite (funs_new_new_constrs new_constr_name gamma_valid pd pdf pf (idents_of_context gamma))
+        with (m:=m) (a:=a); auto.
+    + (*Case 2: not constr*)
+      simpl_rep_full. f_equal; [apply UIP_dec, vty_eq_dec|]. apply dom_cast_eq'.
+      unfold funs_new_full. rewrite funs_new_old_names.
+      2: { apply (sig_f_in_idents gamma (s_name f1)). rewrite in_map_iff. exists f1; split; auto.
+        inversion Hty1; auto.
+      }
+      f_equal.
+      (*Show arg lists equal*)
+      apply get_arg_list_ext; [solve_len|].
+      simpl_len. intros i Hi ty1 Hty3 Hty4.
+      revert Hty3.
+      rewrite map_nth_inbound with (d2:=tm_d); auto. intros Hty3.
+      assert (Hin: In (nth i tms tm_d) tms) by (apply nth_In; auto).
+      rewrite Forall_forall in IH. apply IH; auto.
+  - (*Tlet*)
+    intros tm1 v tm2 IH1 IH2 ty Hty1. simpl. unfold is_true; rewrite !andb_true_iff.
+    intros [Hsimp1 Hsimp2] [Hexh1 Hexh2] Hty2 vv. simpl_rep_full.
+    erewrite tm_change_vv. apply IH2; auto.
+    intros x Hinx.
+    unfold substi. destruct (vsymbol_eq_dec x v); subst; auto. simpl.
+    apply IH1; auto.
+  - (*Tif*)
+    intros f t1 t2 IH1 IH2 IH3 ty Hty1. simpl.
+    unfold is_true; rewrite !andb_true_iff; intros [[Hsimp1 Hsimp2] Hsimp3] [[Hexh1 Hexh2] Hexh3] Hty2 vv. 
+    simpl; simpl_rep_full.
+    rewrite IH1 with (Hty1:=(proj2' (proj2' (ty_if_inv Hty1)))) by auto.
+    rewrite IH2 with (Hty1:=(proj1' (ty_if_inv Hty1)))by auto.
+    rewrite IH3 with (Hty1:=(proj1' (proj2' (ty_if_inv Hty1)))) by auto. 
+    reflexivity.
+  - (*Tmatch*)
+    intros tm ty1 ps IH1 IH2 ty Hty1. simpl. unfold is_true; rewrite !andb_true_iff.
+    intros [[Hsimp1 Hsimp2] Hsimppat] [[Hsimpexh Hex1] Hex2] Hty2 vv.
+    destruct (ty_match_inv Hty1) as [Hty1' [Hallpat Hallty]].
+    (*Know the type is an ADT*)
+    destruct (simple_pat_match_adt gamma_valid true ty Hsimppat Hty1) as 
+    [m [a [m_in [a_in [args [Hargslen [Hvalargs Htyeq]]]]]]].
+    assert (Hallsimp: forallb simple_pat (map fst ps)). {
+      unfold simple_pat_match in Hsimppat. rewrite !andb_true_iff in Hsimppat; apply Hsimppat.
+    }
+    (*Handle inductive case - TODO OK to fix ty?*)
+    assert (IH2': Forall (fun x => forall (Hty1 : term_has_type gamma (snd x) ty),
+         forall
+           (Hty2 : term_has_type new_gamma
+                     (rewriteT keep_muts new_constr_name badnames gamma badvars (snd x)) ty)
+           (vv : val_vars pd vt),
+         term_rep new_gamma_valid pd new_pdf vt new_pf vv
+           (rewriteT keep_muts new_constr_name badnames gamma badvars (snd x)) ty Hty2 =
+         term_rep gamma_valid pd pdf vt pf vv (snd x) ty Hty1) ps).
+    {
+      rewrite forallb_forall in Hsimp2, Hex2.
+      rewrite Forall_map in IH2.
+      rewrite Forall_forall in Hallty, IH2 |- *.
+      intros x Hinx Hty3 Hty4 vv1. apply IH2; auto.
+    }
+    (*Now case on whether or not we encode the type*)
+    revert Hty2.
+    destruct (enc_ty keep_muts gamma ty1) eqn : Henc.
+    2: {
+      (*Here, both are match cases, need to show equivalence between mut in contexts (bc we dont encode)*)
+      intros Hty2.
+      simpl_rep_full.
+      rewrite IH1 with (Hty1:=(proj1' (ty_match_inv Hty1))) by auto.
+      (*Prove that m is in new gamma*)
+      assert (m_in2: mut_in_ctx m new_gamma).
+      {
+        unfold enc_ty in Henc. rewrite Htyeq in Henc. unfold keep_tys in Henc.
+        assert (Hts: find_ts_in_ctx gamma (adt_name a) = Some (m, a)).
+        { apply find_ts_in_ctx_iff; auto. }
+        rewrite Hts in Henc. unfold mut_in_ctx, new_gamma, new_ctx.
+        rewrite fold_all_ctx_gamma_gen_muts. apply In_in_bool, in_filter.
+        apply in_bool_In in m_in; split; auto.
+        destruct (keep_muts m); auto. 
+      }
+      apply match_rep_simple with (b1:=true)(m:=m)(a:=a)(args:=args); auto.
+      - rewrite map_map. simpl. reflexivity.
+      - (*Prove forall*) rewrite map_map. simpl.
+        clear -IH2'. induction ps as [| phd ptl IH]; simpl; auto.
+        inversion IH2'; subst. constructor; auto.
+      - rewrite map_map. simpl. auto.
+    } 
+    
